messageInvariantPrototypes/ringLeaderElection/automate/messageInvariants.dfy
@@ -8,18 +8,10 @@ import opened UtilitiesLibrary
 import opened DistributedSystem
 import opened Obligations
 
-// All msg have a valid ringPos as src
-ghost predicate VoteMsgValidSrc(c: Constants, v: Variables)
-  requires v.WF(c)
-{
-  forall msg | msg in v.network.sentMsgs
-  :: c.ValidIdx(msg.src)
-}
-
 // Every message is sent according to a fixed function
-ghost predicate TransmissionValidity(c: Constants, v: Variables)
+ghost predicate SendMsgValidity(c: Constants, v: Variables)
   requires v.WF(c)
-  requires VoteMsgValidSrc(c, v)
+  requires ValidMessages(c, v)
 {
   forall msg | msg in v.network.sentMsgs
   :: 
@@ -32,17 +24,15 @@ ghost predicate TransmissionValidity(c: Constants, v: Variables)
 ghost predicate MessageInv(c: Constants, v: Variables)
 {
   && v.WF(c)
-  && ValidHistory(c, v)
-  && VoteMsgValidSrc(c, v)
-  && TransmissionValidity(c, v)
-  // && ReceiveValidity(c, v)
+  && ValidVariables(c, v)
+  && SendMsgValidity(c, v)
 }
 
 lemma InitImpliesMessageInv(c: Constants, v: Variables)
   requires Init(c, v)
   ensures MessageInv(c, v)
 {
-  InitImpliesValidHistory(c, v);
+  InitImpliesValidVariables(c, v);
 }
 
 lemma MessageInvInductive(c: Constants, v: Variables, v': Variables)
@@ -50,8 +40,8 @@ lemma MessageInvInductive(c: Constants, v: Variables, v': Variables)
   requires Next(c, v, v')
   ensures MessageInv(c, v')
 {
-  InvNextValidHistory(c, v, v');
-  InvNextTransmissionValidity(c, v, v');
+  InvNextValidVariables(c, v, v');
+  InvNextSendMsgValidity(c, v, v');
 }
 
 
@@ -59,12 +49,12 @@ lemma MessageInvInductive(c: Constants, v: Variables, v': Variables)
 *                                         Proofs                                       *
 ***************************************************************************************/
 
-lemma InvNextTransmissionValidity(c: Constants, v: Variables, v': Variables)
+lemma InvNextSendMsgValidity(c: Constants, v: Variables, v': Variables)
   requires v.WF(c)
-  requires VoteMsgValidSrc(c, v)
-  requires TransmissionValidity(c, v)
+  requires ValidMessages(c, v)
+  requires SendMsgValidity(c, v)
   requires Next(c, v, v')
-  ensures TransmissionValidity(c, v')
+  ensures SendMsgValidity(c, v')
 {
   forall msg | msg in v'.network.sentMsgs
   ensures
